src/goose_lang/lib/encoding/encoding.v
@@ -5,7 +5,7 @@ From Perennial.goose_lang Require Export
      lang notation array typing struct
      tactics lifting proofmode.
 From Perennial.goose_lang Require Import slice basic_triples.
-From Perennial.goose_lang Require Export encoding.
+From Perennial.goose_lang.lib Require Export encoding.impl.
 
 Set Default Proof Using "Type".
 
