src/goose_lang/lib/slice/impl.v
@@ -49,9 +49,6 @@ Section goose_lang.
   Definition Var' s : @expr ext := Var s.
   Local Coercion Var' : string >-> expr.
 
-(** allocation with a type annotation *)
-Definition ref_to (t:ty): val := λ: "v", Alloc "v".
-
 Definition raw_slice (t: ty): val :=
   λ: "p" "sz",
   ("p", "sz", "sz").
