src/goose_lang/lib/struct/struct.v
@@ -1,0 +1,9 @@
+From Perennial.goose_lang Require Import notation typing.
+From Perennial.goose_lang Require Import lifting.
+From Perennial.goose_lang.lib Require Import map.impl.
+
+Section goose_lang.
+  Context {ext:ext_op}.
+  Context {ext_ty:ext_types ext}.
+
+End goose_lang.
