src/goose_lang/lib/typed_mem.v
@@ -1,0 +1,270 @@
+From Perennial.goose_lang Require Export notation typing.
+From Perennial.goose_lang Require Import lifting proofmode.
+From Perennial.goose_lang.lib Require Import map.impl.
+
+Set Default Proof Using "Type".
+
+Section goose_lang.
+  Context `{ffi_sem: ext_semantics} `{!ffi_interp ffi} `{!heapG Σ}.
+  Context {ext_ty: ext_types ext}.
+
+  Inductive lit_ty : base_lit -> ty -> Prop :=
+  | int_ty x : lit_ty (LitInt x) uint64T
+  | int32_ty x : lit_ty (LitInt32 x) uint32T
+  | int8_ty x : lit_ty (LitByte x) byteT
+  | bool_ty x : lit_ty (LitBool x) boolT
+  | string_ty x : lit_ty (LitString x) stringT
+  | unit_ty : lit_ty LitUnit unitT
+  | loc_array_ty x t : lit_ty (LitLoc x) (arrayT t)
+  | loc_struct_ty x ts : lit_ty (LitLoc x) (structRefT ts)
+  .
+
+  (* approximate types for closed values *)
+  Inductive val_ty : val -> ty -> Prop :=
+  | base_ty l t : lit_ty l t -> val_ty (LitV l) t
+  | val_ty_pair v1 t1 v2 t2 : val_ty v1 t1 ->
+                              val_ty v2 t2 ->
+                              val_ty (PairV v1 v2) (prodT t1 t2)
+  | sum_ty_l v1 t1 t2 : val_ty v1 t1 ->
+                        val_ty (InjLV v1) (sumT t1 t2)
+  | sum_ty_r v2 t1 t2 : val_ty v2 t2 ->
+                        val_ty (InjRV v2) (sumT t1 t2)
+  | map_def_ty v t : val_ty v t ->
+                     val_ty (MapNilV v) (mapValT t)
+  | map_cons_ty k v mv' t : val_ty mv' (mapValT t) ->
+                            val_ty k uint64T ->
+                            val_ty v t ->
+                            val_ty (InjRV (k, v, mv')%V) (mapValT t)
+  | rec_ty f x e t1 t2 : val_ty (RecV f x e) (arrowT t1 t2)
+  | ext_def_ty x : val_ty (ExtV (val_ty_def x)) (extT x)
+  .
+
+  Theorem zero_val_ty' t : val_ty (zero_val t) t.
+  Proof.
+    induction t; simpl; eauto using val_ty, lit_ty.
+    destruct t; eauto using val_ty, lit_ty.
+  Qed.
+
+  Ltac invc H := inversion H; subst; clear H.
+
+  Ltac inv_ty :=
+    repeat match goal with
+           | [ H: val_ty _ ?t |- _ ] =>
+             first [ is_var t; fail 1 | invc H ]
+           | [ H: lit_ty _ ?t |- _ ] =>
+             first [ is_var t; fail 1 | invc H ]
+           end.
+
+  Theorem val_ty_len {v t} :
+    val_ty v t ->
+    length (flatten_struct v) = Z.to_nat (ty_size t).
+  Proof.
+    induction 1; simpl; rewrite -> ?app_length in *; auto.
+    - invc H; eauto.
+    - pose proof (ty_size_ge_0 t1).
+      pose proof (ty_size_ge_0 t2).
+      lia.
+  Qed.
+
+  Theorem val_ty_flatten_length v t :
+    val_ty v t ->
+    length (flatten_struct v) = length (flatten_ty t).
+  Proof.
+    induction 1; simpl; auto.
+    - invc H; eauto.
+    - rewrite ?app_length.
+      lia.
+  Qed.
+
+  Theorem ty_size_offset t l j :
+    l +ₗ (length (flatten_ty t) + j)%nat = l +ₗ ty_size t +ₗ j.
+  Proof.
+    rewrite loc_add_assoc.
+    f_equal.
+    rewrite <- ty_size_length.
+    pose proof (ty_size_ge_0 t).
+    lia.
+  Qed.
+
+  Definition struct_mapsto l q (t:ty) (v: val): iProp Σ :=
+    (([∗ list] j↦vj ∈ flatten_struct v, (l +ₗ j) ↦{q} vj) ∗ ⌜val_ty v t⌝)%I.
+
+  Notation "l ↦[ t ]{ q } v" := (struct_mapsto l q t v%V)
+                                   (at level 20, q at level 50, t at level 50,
+                                    format "l  ↦[ t ]{ q }  v") : bi_scope.
+  Notation "l ↦[ t ] v" := (struct_mapsto l 1 t v%V)
+                              (at level 20, t at level 50,
+                               format "l  ↦[ t ]  v") : bi_scope.
+
+  Theorem struct_mapsto_singleton l q t v v0 :
+    flatten_struct v = [v0] ->
+    l ↦[t]{q} v -∗ l ↦{q} v0.
+  Proof.
+    intros Hv.
+    rewrite /struct_mapsto Hv /=.
+    rewrite loc_add_0 right_id.
+    by iIntros "[$ _]".
+  Qed.
+
+  Fixpoint load_ty t: val :=
+    match t with
+    | prodT t1 t2 => λ: "l", (load_ty t1 (Var "l"), load_ty t2 (Var "l" +ₗ[t1] #1))
+    | baseT unitBT => λ: <>, #()
+    | _ => λ: "l", !(Var "l")
+    end.
+
+  Fixpoint store_ty t: val :=
+    match t with
+    | prodT t1 t2 => λ: "p" "v",
+                    store_ty t1 (Var "p") (Fst (Var "v"));;
+                    store_ty t2 (Var "p" +ₗ[t1] #1) (Snd (Var "v"))
+    | baseT unitBT => λ: <> <>, #()
+    | _ => λ: "p" "v", Var "p" <- Var "v"
+    end.
+
+  Lemma wp_LoadAt stk E q l t v :
+    {{{ l ↦[t]{q} v }}}
+      load_ty t #l @ stk; E
+    {{{ RET v; l ↦[t]{q} v }}}.
+  Proof.
+    iIntros (Φ) "Hl HΦ".
+    iDestruct "Hl" as "[Hl %]".
+    hnf in H.
+    iAssert (▷ (([∗ list] j↦vj ∈ flatten_struct v, (l +ₗ j)↦{q} vj) -∗ Φ v))%I with "[HΦ]" as "HΦ".
+    { iIntros "!> HPost".
+      iApply "HΦ".
+      iSplit; eauto. }
+    (* TODO: we have to rename this so it doesn't conflict with a name generated
+  by induction; seems like a bug *)
+    rename l into l'.
+    (iInduction H as [ | | | | | | | ] "IH" forall (l' Φ));
+      simpl;
+      wp_pures;
+      rewrite ?loc_add_0 ?right_id.
+    - inversion H; subst; simpl;
+        rewrite ?loc_add_0 ?right_id;
+        try wp_apply (wp_load with "[$]"); auto.
+      wp_pures.
+      iApply ("HΦ" with "[//]").
+    - rewrite big_opL_app.
+      iDestruct "Hl" as "[Hv1 Hv2]".
+      wp_apply ("IH" with "Hv1"); iIntros "Hv1".
+      wp_apply ("IH1" with "[Hv2]"); [ | iIntros "Hv2" ].
+      { erewrite val_ty_flatten_length; eauto.
+        setoid_rewrite ty_size_offset.
+        rewrite Z.mul_1_r.
+        iFrame. }
+      wp_pures.
+      iApply "HΦ"; iFrame.
+      erewrite val_ty_flatten_length by eauto.
+      setoid_rewrite ty_size_offset.
+      rewrite Z.mul_1_r.
+      iFrame.
+    - wp_apply (wp_load with "[$]"); auto.
+    - wp_apply (wp_load with "[$]"); auto.
+    - wp_apply (wp_load with "[$]"); auto.
+    - wp_apply (wp_load with "[$]"); auto.
+    - wp_apply (wp_load with "[$]"); auto.
+    - wp_apply (wp_load with "[$]"); auto.
+  Qed.
+
+  Lemma wp_store stk E l v v' :
+    {{{ ▷ l ↦ v' }}} Store (Val $ LitV (LitLoc l)) (Val v) @ stk; E
+    {{{ RET LitV LitUnit; l ↦ v }}}.
+  Proof.
+    iIntros (Φ) "Hl HΦ". rewrite /Store.
+    wp_apply (wp_prepare_write with "Hl"); iIntros "Hl".
+    by wp_apply (wp_finish_store with "Hl").
+  Qed.
+
+  Lemma wp_StoreAt stk E l t v0 v :
+    val_ty v t ->
+    {{{ l ↦[t] v0 }}}
+      store_ty t #l v @ stk; E
+    {{{ RET #(); l ↦[t] v }}}.
+  Proof.
+    intros Hty.
+    iIntros (Φ) "[Hl %] HΦ".
+    iAssert (▷ (([∗ list] j↦vj ∈ flatten_struct v, (l +ₗ j)↦ vj) -∗ Φ #()))%I with "[HΦ]" as "HΦ".
+    { iIntros "!> HPost".
+      iApply "HΦ".
+      iSplit; eauto. }
+    rename v into v'.
+    rename l into l'.
+    (iInduction H as [ | | | | | | | ] "IH" forall (v' Hty l' Φ));
+      simpl;
+      rewrite ?loc_add_0 ?right_id;
+      wp_pures.
+    - invc Hty; invc H;
+        try match goal with
+            | [ H: lit_ty _ _ |- _ ] => invc H
+            end;
+        simpl;
+        rewrite ?loc_add_0 ?right_id;
+        try (wp_apply (wp_store with "[$]"); auto).
+      wp_pures.
+      iApply ("HΦ" with "[//]").
+    - rewrite big_opL_app.
+      erewrite val_ty_flatten_length by eauto.
+      setoid_rewrite ty_size_offset.
+      invc Hty.
+      { by invc H1. (* can't be a pair and a base literal *) }
+      iDestruct "Hl" as "[Hv1 Hv2]".
+      wp_pures.
+      wp_apply ("IH" with "[//] Hv1").
+      iIntros "Hv1".
+      wp_pures.
+      rewrite Z.mul_1_r.
+      wp_apply ("IH1" with "[//] Hv2").
+      iIntros "Hv2".
+      iApply "HΦ".
+      simpl.
+      rewrite big_opL_app.
+      iFrame.
+      erewrite val_ty_flatten_length by eauto.
+      setoid_rewrite ty_size_offset.
+      iFrame.
+    - inv_ty;
+        rewrite /= ?loc_add_0 ?right_id;
+        wp_apply (wp_store with "[$]"); auto.
+    - inv_ty;
+        rewrite /= ?loc_add_0 ?right_id;
+        wp_apply (wp_store with "[$]"); auto.
+    - invc Hty;
+        try match goal with
+            | [ H: lit_ty _ _ |- _ ] => invc H
+            end;
+        rewrite /= ?loc_add_0 ?right_id;
+        wp_apply (wp_store with "[$]"); auto.
+    - invc Hty;
+        try match goal with
+            | [ H: lit_ty _ _ |- _ ] => invc H
+            end;
+        rewrite /= ?loc_add_0 ?right_id;
+        wp_apply (wp_store with "[$]"); auto.
+    - inv_ty;
+        rewrite /= ?loc_add_0 ?right_id;
+        wp_apply (wp_store with "[$]"); auto.
+    - inv_ty;
+        rewrite /= ?loc_add_0 ?right_id;
+        wp_apply (wp_store with "[$]"); auto.
+  Qed.
+
+End goose_lang.
+
+Ltac val_ty :=
+  lazymatch goal with
+  | |- val_ty (zero_val _) _ => apply zero_val_ty'
+  | [ H: val_ty ?v ?t |- val_ty ?v ?t ] => exact H
+  | |- val_ty _ _ => solve [ repeat constructor ]
+  | _ => fail "not a val_ty goal"
+  end.
+
+Hint Extern 2 (val_ty _ _) => val_ty : core.
+
+Notation "l ↦[ ty ]{ q } v" := (struct_mapsto l q ty v%V)
+                                 (at level 20, q at level 50, ty at level 50,
+                                  format "l  ↦[ ty ]{ q }  v") : bi_scope.
+Notation "l ↦[ ty ] v" := (struct_mapsto l 1 ty v%V)
+                            (at level 20, ty at level 50,
+                             format "l  ↦[ ty ]  v") : bi_scope.
